examples/dynamic_isolation/Proof.v
@@ -4,6 +4,7 @@ Require Import Coq.Lists.List.
 Require Import Koika.Std.
 
 Require Import dynamic_isolation.Interfaces.
+Require Import dynamic_isolation.LogHelpers.
 Require Import dynamic_isolation.External.
 Require Import dynamic_isolation.Multicore.
 
@@ -24,7 +25,7 @@ Module Pf (External: External_sig) (EnclaveParams: EnclaveParameters)
 
   Record enclave_params :=
     { metadata : enclave_metadata;
-      param_dram: initial_dram_t
+      param_dram: dram_t
     }.
 
   Record core_config : Type :=
@@ -39,8 +40,8 @@ Module Pf (External: External_sig) (EnclaveParams: EnclaveParameters)
   Definition isolated_function_t : Type := ind_core_id -> enclave_params -> rf_t -> nat -> observations_t.
 
   Record partitioned_memory :=
-    { pm_enclave_mem : enclave_id -> option initial_dram_t;
-      pm_shared_page : option initial_dram_t;
+    { pm_enclave_mem : enclave_id -> option dram_t;
+      pm_shared_page : option dram_t;
     }.
 
   Record ghost_state :=
@@ -66,23 +67,23 @@ Module Pf (External: External_sig) (EnclaveParams: EnclaveParameters)
   Definition enclave_max enc_id := Bits.to_nat (Bits.plus (EnclaveParams.enclave_base enc_id)
                                                           (EnclaveParams.enclave_size enc_id)).
 
-  Definition initial_enclave_dram initial_dram enc_id : initial_dram_t :=
+  Definition initial_enclave_dram initial_dram enc_id : dram_t :=
     fun addr => if ((enclave_base enc_id) <=? addr) && (addr <? (enclave_max enc_id))
              then initial_dram addr
              else None.
 
-  Definition initial_shared_mem initial_dram : initial_dram_t :=
+  Definition initial_shared_mem initial_dram : dram_t :=
     fun addr => if ((Bits.to_nat (EnclaveParams.shared_mem_base) <=? addr) &&
                  (addr <? Bits.to_nat (Bits.plus EnclaveParams.shared_mem_base EnclaveParams.shared_mem_size)))
              then initial_dram addr
              else None.
 
-  Definition mk_initial_pm (initial_dram: initial_dram_t) : partitioned_memory :=
+  Definition mk_initial_pm (initial_dram: dram_t) : partitioned_memory :=
     {| pm_enclave_mem := fun eid => Some (initial_enclave_dram initial_dram eid);
        pm_shared_page := Some (initial_shared_mem initial_dram)
     |}.
 
-  Definition initial_ghost_state (fn: isolated_function_t) (initial_dram: initial_dram_t) : ghost_state :=
+  Definition initial_ghost_state (fn: isolated_function_t) (initial_dram: dram_t) : ghost_state :=
     let enclave0_param :=
         {| metadata := {| meta_eid := Enclave0;
                           shared_page := false
@@ -108,7 +109,7 @@ Module Pf (External: External_sig) (EnclaveParams: EnclaveParameters)
 
   (* TODO: Do we care about cycle-accurate purge? *)
   Inductive function_generates_trace_helper
-            (fn: isolated_function_t) (initial_dram: initial_dram_t)
+            (fn: isolated_function_t) (initial_dram: dram_t)
             (ghost: ghost_state) (tr: trace) : Prop :=
   | EmptyTrace :
       forall (initial_ghost : ghost = initial_ghost_state fn initial_dram)
@@ -150,12 +151,12 @@ Module Pf (External: External_sig) (EnclaveParams: EnclaveParameters)
 
 
 
-  Definition function_generates_trace (fn: isolated_function_t) (initial_dram: initial_dram_t) (tr: trace) : Prop :=
+  Definition function_generates_trace (fn: isolated_function_t) (initial_dram: dram_t) (tr: trace) : Prop :=
     exists ghost_state, function_generates_trace_helper fn initial_dram ghost_state tr.
 
 
   Section Initialised.
-    Variable initial_dram: initial_dram_t.
+    Variable initial_dram: dram_t.
 
     Theorem simulation: exists (iso_fn : isolated_function_t),
       forall (n: nat) (impl_st: Impl.state) (impl_tr: trace),
@@ -168,6 +169,365 @@ Module Pf (External: External_sig) (EnclaveParams: EnclaveParameters)
 End Pf.
 *)
 
+Module SMProperties (External: External_sig) (Params: EnclaveParameters).
+  Module SM := SecurityMonitor External Params.
+  Include SM.
+  Import Interfaces.Common.
+  Import Interfaces.EnclaveInterface.
+
+  Section Semantics.
+    Definition empty_log : Log R ContextEnv := log_empty.
+    Parameter update_function : state -> Log R ContextEnv -> Log R ContextEnv.
+      (* interp_scheduler' st ? rules log scheduler. *)
+
+  End Semantics.
+
+  Section LogHelpers.
+    Definition update_no_writes_to_reg (st: state) (log: Log R ContextEnv) (reg: reg_t) : Prop :=
+      latest_write (update_function st log) reg = latest_write log reg.
+
+  End LogHelpers.
+
+  Section ValidInput.
+    Definition valid_input_log (log: Log R ContextEnv) : Prop. Admitted.
+    Definition valid_input_state (st: state) : Prop. Admitted.
+    Definition valid_feedback_log : state -> Log R ContextEnv -> Log R ContextEnv -> Prop. Admitted.
+
+    Definition internal_reg_to_taint (reg: internal_reg_t) : option ind_core_id :=
+      match reg with
+      | limbo0 => Some CoreId0
+      | limbo1 => Some CoreId1
+      | enc_data0 => Some CoreId0
+      | enc_data1 => Some CoreId1
+      end.
+
+    Definition reg_to_taint (reg: reg_t) : option ind_core_id :=
+      match reg with
+      | fromCore0_IMem st => Some CoreId0
+      | fromCore0_DMem st => Some CoreId0
+      | fromCore0_Enc st => Some CoreId0
+      | toCore0_IMem st => Some CoreId0
+      | toCore0_DMem st => Some CoreId0
+      (* Core1 <-> SM *)
+      | fromCore1_IMem st => Some CoreId1
+      | fromCore1_DMem st => Some CoreId1
+      | fromCore1_Enc st => Some CoreId1
+      | toCore1_IMem st => Some CoreId1
+      | toCore1_DMem st => Some CoreId1
+      (* SM <-> Mem *)
+      | toMem0_IMem st => Some CoreId0
+      | toMem0_DMem st => Some CoreId0
+      | toMem1_IMem st => Some CoreId1
+      | toMem1_DMem st => Some CoreId1
+      | fromMem0_IMem st => Some CoreId0
+      | fromMem0_DMem st => Some CoreId0
+      | fromMem1_IMem st => Some CoreId1
+      | fromMem1_DMem st => Some CoreId1
+      | pc_core0 => Some CoreId0
+      | pc_core1 => Some CoreId1
+      | purge_core0 => Some CoreId0
+      | purge_core1 => Some CoreId1
+      | purge_mem0 => Some CoreId0
+      | purge_mem1 => Some CoreId1
+      | internal st => internal_reg_to_taint st
+    end.
+
+  End ValidInput.
+
+  Section Initialise.
+
+    Definition initialise_internal_with_eid
+               (eid0: option enclave_id) (eid1: option enclave_id) (idx: internal_reg_t) : R_internal idx :=
+      match idx with
+      | limbo0 => Ob~0
+      | limbo1 => Ob~0
+      | enc_data0 =>
+         match eid0 with
+         | Some id => eid_to_initial_enclave_data id
+         | None => value_of_bits (Bits.zero)
+         end
+      | enc_data1 =>
+         match eid1 with
+         | Some id => eid_to_initial_enclave_data id
+         | None => value_of_bits (Bits.zero)
+         end
+      end.
+
+    Definition initialise_with_eid (eid0: option enclave_id) (eid1: option enclave_id) (idx: reg_t) : R idx :=
+      match idx with
+      | internal s => initialise_internal_with_eid eid0 eid1 s
+      | s => r s
+      end.
+
+  End Initialise.
+
+  Section ValidResetState.
+
+    (* TODO: not quite complete. *)
+    Definition valid_reset_state (st: state) (core_id: ind_core_id) (eid: enclave_id): Prop :=
+      forall reg, reg_to_taint reg = Some core_id ->
+             (reg <> pc_core0 /\ reg <> pc_core1) ->
+             match core_id with
+             | CoreId0 => initialise_with_eid (Some eid) None reg = ContextEnv.(getenv) st reg
+             | CoreId1 => initialise_with_eid None (Some eid) reg = ContextEnv.(getenv) st reg
+             end.
+
+  End ValidResetState.
+
+  Section SMInternalAxioms.
+
+    Definition valid_enclave_data (data: struct_t enclave_data) : Prop :=
+      let enclave_data := extract_enclave_data data in
+      match bits_id_to_ind_id enclave_data.(enclave_data_eid) with
+      | Some id =>
+          enclave_data.(enclave_data_addr_min) = Params.enclave_base id /\
+          enclave_data.(enclave_data_size) = Params.enclave_size id
+      | None => False
+      end.
+
+    Definition valid_enclave_data_regs (st: state) : Prop :=
+      valid_enclave_data (ContextEnv.(getenv) st (internal enc_data0)) /\
+      valid_enclave_data (ContextEnv.(getenv) st (internal enc_data1)).
+
+    (* TODO: incomplete *)
+    Definition valid_internal_state (st: state) : Prop :=
+      valid_enclave_data_regs st.
+
+    Definition limbo_eq (st: state) (core_id: ind_core_id) (v: bits_t 1): Prop :=
+      match core_id with
+      | CoreId0 => ContextEnv.(getenv) st (internal limbo0) = v
+      | CoreId1 => ContextEnv.(getenv) st (internal limbo1) = v
+      end.
+
+    (* Idea:
+     * - ghost state tracks when cores are done purging and when cores have restarted?
+     * - or we explicitly add it to the observations! <-- This seems better, since it defines what we care about
+     *)
+
+    Definition equiv_log_at_core (core_id: ind_core_id) (log1: Log R ContextEnv) (log2: Log R ContextEnv) : Prop :=
+      forall r, reg_to_taint r = Some core_id ->
+           ContextEnv.(getenv) log1 r = ContextEnv.(getenv) log2 r.
+
+    Definition equiv_log_at_shared (log1: Log R ContextEnv) (log2: Log R ContextEnv) : Prop :=
+      forall r, reg_to_taint r = None ->
+           ContextEnv.(getenv) log1 r = ContextEnv.(getenv) log2 r.
+
+    Definition equiv_log_for_core (core_id: ind_core_id) (log1: Log R ContextEnv) (log2: Log R ContextEnv) : Prop :=
+      equiv_log_at_core core_id log1 log2 /\ equiv_log_at_shared log1 log2.
+
+    Definition equiv_st_at_core (core_id: ind_core_id) (st1: state) (st2: state) : Prop :=
+      forall r, reg_to_taint r = Some core_id ->
+           ContextEnv.(getenv) st1 r = ContextEnv.(getenv) st2 r.
+
+    Definition equiv_st_at_shared (st1: state) (st2: state) : Prop :=
+      forall r, reg_to_taint r = None ->
+           ContextEnv.(getenv) st1 r = ContextEnv.(getenv) st2 r.
+
+    Definition equiv_st_for_core (core_id: ind_core_id) (st1: state) (st2: state) : Prop :=
+      equiv_st_at_core core_id st1 st2 /\ equiv_st_at_shared st1 st2.
+
+    (* Assuming we are not initially in a limbo state, output is a function only of taint0 registers *)
+    Definition output_is_a_function_of_partitioned_registers:
+      forall (core_id: ind_core_id) (st0 st1: state) (log0 log1: Log R ContextEnv),
+      limbo_eq st0 core_id Ob~0 ->
+      valid_input_state st0 ->
+      valid_input_state st1 ->
+      valid_input_log log0 ->
+      valid_input_log log1 ->
+      equiv_st_for_core core_id st0 st1 ->
+      equiv_log_for_core core_id log0 log1 ->
+      equiv_log_for_core core_id (update_function st0 log0) (update_function st1 log1).
+    Admitted.
+
+    (* TODO: figure out dependent types *)
+    Definition no_enq_to_output_reg (core_id: ind_core_id) (reg: reg_t) (log: Log R ContextEnv): Prop :=
+      match reg with
+      | toCore0_IMem MemResp.valid0 =>
+          core_id = CoreId0 /\
+          latest_write log (toCore0_IMem MemResp.valid0) <> Some Ob~1
+      | toCore0_DMem MemResp.valid0 =>
+          core_id = CoreId0 /\
+          latest_write log (toCore0_DMem MemResp.valid0) <> Some Ob~1
+      | toMem0_IMem MemReq.valid0 =>
+          core_id = CoreId0 /\
+          latest_write log (toMem0_IMem MemReq.valid0) <> Some Ob~1
+      | toMem0_DMem MemReq.valid0 =>
+          core_id = CoreId0 /\
+          latest_write log (toMem0_DMem MemReq.valid0) <> Some Ob~1
+      | toCore1_IMem MemResp.valid0 =>
+          core_id = CoreId1 /\
+          latest_write log (toCore1_IMem MemResp.valid0) <> Some Ob~1
+      | toCore1_DMem MemResp.valid0 =>
+          core_id = CoreId1 /\
+          latest_write log (toCore1_DMem MemResp.valid0) <> Some Ob~1
+      | toMem1_IMem MemReq.valid0 =>
+          core_id = CoreId1 /\
+          latest_write log (toMem1_IMem MemReq.valid0) <> Some Ob~1
+      |toMem1_DMem MemReq.valid0 =>
+          core_id = CoreId1 /\
+          latest_write log (toMem1_DMem MemReq.valid0) <> Some Ob~1
+      | _ => False
+      end.
+
+    (* TODO: rephrase this. This is annoying to work with *)
+    Definition no_external_enqs (core_id: ind_core_id) (st: state) (log: Log R ContextEnv) : Prop :=
+      forall reg, no_enq_to_output_reg core_id reg (update_function st log) \/
+             update_no_writes_to_reg st log reg.
+
+    (* If the core starts out in a limbo state, we say there are no valid writes to the outside world *)
+    Definition limbo_implies_no_external_enqs:
+      forall (core_id: ind_core_id) (st: state) (log: Log R ContextEnv),
+      limbo_eq st core_id Ob~1 ->
+      valid_input_state st ->
+      valid_input_log log ->
+      no_external_enqs core_id st log.
+    Proof.
+    Admitted.
+  End SMInternalAxioms.
+
+  (* TODO: this needs to be in a framework *)
+  Section CycleModel.
+    Variable input_fn : state -> Log R ContextEnv.
+    Variable pf_input_fn_generates_valid_log : forall (st: state), valid_input_log (input_fn st).
+    Variable feedback_fn : state -> Log R ContextEnv -> Log R ContextEnv.
+    Variable pf_feedback_fn_generates_valid_log
+      : forall (st: state) (log: Log R ContextEnv), valid_feedback_log st log (feedback_fn st log).
+
+    Definition do_step (st: state) : state :=
+      let input := input_fn st in
+      let update := update_function st input in
+      let final := feedback_fn st update in
+      commit_update st final.
+
+    (* Model cycle with input, schedule, post-schedule update
+     * Important points
+     * - From a reset state, requests to memory are a function only of inputs to relevant core,
+     *   until a context switch is requested
+     * - All requests to memory are within range of the enclave
+     * - When a context switch is requested, we have no more requests to memory
+     * - Need something about how the time it takes for memory/core to reset is independent...,
+     *   but that's not here
+     *)
+
+    Definition prop_holds_about_sm_step (st: state) (P: state -> Log R ContextEnv -> Log R ContextEnv -> Prop) : Prop :=
+      let input := input_fn st in
+      let update := update_function st input in
+      P st input update.
+
+    Fixpoint prop_holds_for_n_sm_steps (n: nat) (st: state) (P: state -> Log R ContextEnv -> Log R ContextEnv -> Prop) : Prop :=
+      match n with
+      | 0 => True
+      | S n' =>
+        let state' := do_step st in
+        prop_holds_about_sm_step st P /\
+        prop_holds_for_n_sm_steps n' state' P
+      end.
+
+    Definition P_partition (core_id: ind_core_id)
+               (st: state) (input_log: Log R ContextEnv) (output_log: Log R ContextEnv) : Prop :=
+      forall st' log',
+      valid_input_state st' ->
+      valid_input_log log' ->
+      equiv_st_for_core core_id st st' ->
+      equiv_log_for_core core_id input_log log' ->
+      equiv_log_for_core core_id output_log (update_function st' log').
+
+    (* TODO: restructure *)
+    Definition observe_enclave_reqs (log: Log R ContextEnv) (core_id: ind_core_id) : option (struct_t enclave_req).
+    Admitted.
+
+    Definition valid_enclave_req (req: struct_t enclave_req) : Prop :=
+      let '(eid, _) := req in
+      Bits.to_nat eid < 4.
+
+    Definition P_no_enclave_req (core_id: ind_core_id): state -> Log R ContextEnv -> Log R ContextEnv -> Prop :=
+      fun st input_log output_log =>
+        match observe_enclave_reqs output_log core_id with
+        | None => True
+        | Some req => valid_enclave_req req
+        end.
+
+    (* TODO: stop duplicating code *)
+    Definition observe_imem_reqs_to_mem0 (log: Log R ContextEnv) : option (struct_t mem_req) :=
+      match latest_write0 log (toMem0_IMem MemReq.valid0) with
+      | Some b =>
+          if Bits.single b then (latest_write0 log (toMem0_IMem MemReq.data0)) else None
+      | None => None
+      end.
+
+    Definition observe_imem_reqs_to_mem1 (log: Log R ContextEnv) : option (struct_t mem_req) :=
+      match latest_write0 log (toMem1_IMem MemReq.valid0) with
+      | Some b =>
+          if Bits.single b then (latest_write0 log (toMem1_IMem MemReq.data0)) else None
+      | None => None
+      end.
+
+    Definition observe_imem_reqs_to_mem (log: Log R ContextEnv) (core_id: ind_core_id) : option (struct_t mem_req) :=
+      match core_id with
+      | CoreId0 => observe_imem_reqs_to_mem0 log
+      | CoreId1 => observe_imem_reqs_to_mem1 log
+      end.
+
+    Definition observe_dmem_reqs_to_mem0 (log: Log R ContextEnv) : option (struct_t mem_req) :=
+      match latest_write0 log (toMem0_DMem MemReq.valid0) with
+      | Some b =>
+          if Bits.single b then (latest_write0 log (toMem0_DMem MemReq.data0)) else None
+      | None => None
+      end.
+
+    Definition observe_dmem_reqs_to_mem1 (log: Log R ContextEnv) : option (struct_t mem_req) :=
+      match latest_write0 log (toMem1_DMem MemReq.valid0) with
+      | Some b =>
+          if Bits.single b then (latest_write0 log (toMem1_DMem MemReq.data0)) else None
+      | None => None
+      end.
+
+    Definition observe_dmem_reqs_to_mem (log: Log R ContextEnv) (core_id: ind_core_id) : option (struct_t mem_req) :=
+      match core_id with
+      | CoreId0 => observe_dmem_reqs_to_mem0 log
+      | CoreId1 => observe_dmem_reqs_to_mem1 log
+      end.
+
+    Definition P_mem_reqs_in_range (mem: ind_cache_type) (core_id: ind_core_id) (eid: enclave_id)
+                                   : state -> Log R ContextEnv -> Log R ContextEnv -> Prop :=
+      let addr_min := Params.enclave_base eid in
+      let addr_max := Bits.plus (Params.enclave_base eid) (Params.enclave_size eid) in
+      fun st input_log output_log =>
+        let req_opt := match mem with
+                       | CacheType_Imem => observe_imem_reqs_to_mem output_log core_id
+                       | CacheType_Dmem => observe_dmem_reqs_to_mem output_log core_id
+                       end in
+        match req_opt with
+        | None => True
+        | Some req =>
+            let addr := mem_req_get_addr req in
+            (Bits.unsigned_le addr_min addr = true) /\ (Bits.unsigned_lt addr addr_max = true)
+        end.
+
+    (* The proof itself is simpler, something like "output_is_a_function_of_partitioned_registers" *)
+    (* TODO: need to include mention of shared state *)
+    Theorem partitioned_when_in_reset_state:
+      forall (core_id: ind_core_id) (st: state) (eid: enclave_id),
+      valid_reset_state st core_id eid ->
+      forall (n: nat),
+      prop_holds_for_n_sm_steps n st (P_no_enclave_req core_id) ->
+      prop_holds_for_n_sm_steps n st (P_partition core_id).
+    Admitted.
+
+    Theorem reqs_to_enclave_memory_in_range:
+      forall (core_id: ind_core_id) (st: state) (eid: enclave_id),
+      valid_reset_state st core_id eid ->
+      forall (n: nat),
+      prop_holds_for_n_sm_steps n st (P_no_enclave_req core_id) ->
+      prop_holds_for_n_sm_steps n st (P_mem_reqs_in_range CacheType_Imem core_id eid) /\
+      prop_holds_for_n_sm_steps n st (P_mem_reqs_in_range CacheType_Dmem core_id eid).
+    Admitted.
+
+    (* TODO: For context switching, state that core output is a function also of the other core's enclave *)
+
+  End CycleModel.
+End SMProperties.
+
 Module TradPf (External: External_sig) (EnclaveParams: EnclaveParameters)
           (Params0: CoreParameters) (Params1: CoreParameters)
           (Core0: Core_sig External EnclaveParams Params0)
@@ -179,7 +539,7 @@ Module TradPf (External: External_sig) (EnclaveParams: EnclaveParameters)
   Import Common.
 
   Section Initialised.
-    Variable initial_dram: initial_dram_t.
+    Variable initial_dram: dram_t.
 
     Theorem simulation: forall (n: nat)
                           (impl_st: Impl.state) (impl_tr: trace)
